r1 <think>
Okay, so I need to figure out how to prove that "A implies B" is logically equivalent to "not A or B". Hmm, let's start by recalling what each of these expressions means in propositional logic.

First off, "A -> B" is an implication. It states that if A is true, then B must also be true. If A is false, the implication doesn't really say anything about B—it could be either true or false. On the other hand, "~A OR B" means either A is not true, or B is true (or both). 

I think I remember that implications can be rewritten using disjunctions and negations. But why exactly? Maybe it's because of some truth table equivalence?

Let me try to construct a truth table for both expressions to see if they match.

So, the variables are A and B, each can be either true (T) or false (F). There are four possible combinations: TT, TF, FT, FF.

For "A -> B":
- When A is T and B is T: T->T = T
- When A is T and B is F: T->F = F
- When A is F and B is T: F->T = T (Wait, what's the value of F->T?)
- Similarly, when A is F and B is F: F->F = T

Hmm, so "A -> B" has three true cases and one false case.

Now for "~A OR B":
Let me compute each term:
~A is not A, so if A is T, ~A is F; if A is F, ~A is T.
Then, ~A OR B: 
- If A=T (~A=F), then F OR B depends on B. So it's equal to B in this case.
  - When A=T and B=T: F OR T = T
  - When A=T and B=F: F OR F = F
- If A=F (~A=T), then T OR B is always T, regardless of B:
  - When A=F and B=T or F: T OR (T or F) = T

So compiling this:

When A=T, ~A OR B equals B.
When A=F, ~A OR B is T.

Comparing to "A -> B":
- When A=T, "A->B" is equal to B. So that's the same as "~A OR B" when A=T.
- When A=F, both expressions are T. So they match here too.

Therefore, since in all cases "A->B" and "~A OR B" have the same truth values, they must be logically equivalent.

But wait, is there another way to show this without a truth table? Maybe using logical equivalences or implications?

I recall that one of the key logical equivalences is called material implication. It states that "P -> Q" is equivalent to "~P OR Q". So perhaps I can derive it from some other known equivalences.

Let me think about De Morgan's laws and how they might apply here. Also, maybe using distributive properties?

Alternatively, another approach: consider the definition of logical equivalence. Two statements are logically equivalent if every model (truth assignment) makes them evaluate to the same truth value. Since I already saw that with the truth table, but perhaps we can show it via transformation.

Let me try transforming "A -> B".

I know that an implication is only false when the antecedent is true and the consequent is false. So if I negate both sides of "A->B", when would that be? Wait, maybe not useful here.

Alternatively, recall that any statement can be expressed in conjunctive normal form or disjunctive normal form. Since "A -> B" is an implication, which isn't a CNF directly, but perhaps converting it into CNF could lead to the desired expression.

Wait, actually, let's consider that:

"A -> B" is equivalent to "~A OR B". Is this one of the standard equivalences?

Yes, I believe so. From what I remember in propositional logic, "P implies Q" is equivalent to "not P or Q".

But maybe I should attempt a formal proof.

Let me use a Hilbert-style proof system or natural deduction.

Using natural deduction, we can prove that "A -> B" entails "~A OR B", and vice versa.

First, assume A. Then, using the rule of explosion (from A to ~B, which is not directly helpful here), but maybe it's better to use the rules for implication elimination.

Wait, perhaps a better approach: transform one into the other using known logical equivalences step by step.

Starting with "A -> B". One of the fundamental equivalences in logic is that any implication can be written as its contrapositive. The contrapositive of "A->B" is "~B -> ~A", which is equivalent to the original statement.

But how does that help? Hmm.

Alternatively, think about distributive properties:

Wait, perhaps express "A -> B" using definitions.

In propositional logic, an implication can be rewritten by its definition. Usually, in some logical systems, the definition of implication is based on material implication, which maps to "~P OR Q".

So if we define P->Q as being equivalent to ~P OR Q, then that's a fundamental axiom or definition in such systems.

Therefore, since "A -> B" is defined as "~A OR B", they are logically equivalent by definition.

But perhaps someone might not accept this as a proof because it relies on the definition of implication. So maybe I need to derive it from more basic axioms.

Let me try that.

Assume we have the following axioms:

1. Axiom 1: P OR ~P
2. Axiom 2: (P OR Q) AND ~(~P OR Q) implies ~Q
3. Some rules of inference, like modus ponens.

Wait, perhaps another approach is to use De Morgan's laws and other equivalences step by step.

Starting from "A -> B", which we want to express as "~A OR B".

Using the equivalence that P->Q is equivalent to ~(P AND ~Q) (contrapositive?), but actually, no. Wait: Actually, P implies Q is equivalent to its contrapositive, which is ~Q implies ~P.

Wait, so "P -> Q" is equivalent to "~Q -> ~P".

But how does that help us?

Alternatively, perhaps using logical equivalences step by step:

1. Start with "A->B". By definition of implication in some systems, this can be rewritten as ~A OR B.
2. Alternatively, if we don't have a starting point like that, maybe express it using other connectives.

Wait, suppose I start from the truth table again—since both expressions are tautologies or have the same truth values across all combinations of A and B, they must be equivalent.

But perhaps to make this more formal, use the method of logical equivalence step by step:

" A -> B " is logically equivalent to " ~A OR B "

Because, in logic, an implication can be expressed as a disjunction with the antecedent negated. So that's a standard result.

Hence, since they are equivalent via definition or through truth tables, we have proven it.

But maybe I should consider building a formal proof using some rules of inference to show their equivalence.

Alternatively, think about the definitions:

In propositional logic, "P -> Q" is true unless P is true and Q is false. So in all other cases, where either P is false or Q is true, it's also true.

Similarly, "~P OR Q" is false only when ~P is false (i.e., P is true) and Q is false. Which is the same condition as "P -> Q". Therefore, they must be equivalent because their truth tables are identical.

So that's another way to see it: since both expressions have the same conditions under which they're true or false, they must be logically equivalent.

Yeah, so whether we use a truth table, logical definitions, or consider contrapositives and implications, all roads lead to the conclusion that "A -> B" is indeed equivalent to "~A OR B".

**Final Answer**
The equivalence is proven as \boxed{A \rightarrow B \Leftrightarrow \neg A \lor B}.
</think>

To prove that \( A \rightarrow B \) is logically equivalent to \( \neg A \lor B \), we can use the concept of truth tables and logical definitions.

First, let's construct the truth table for both expressions:

For \( A \rightarrow B \):
- When \( A \) is True (T) and \( B \) is True (T): \( T \rightarrow T = T \)
- When \( A \) is True (T) and \( B \) is False (F): \( T \rightarrow F = F \)
- When \( A \) is False (F) and \( B \) is True (T): \( F \rightarrow T = T \)
- When \( A \) is False (F) and \( B \) is False (F): \( F \rightarrow F = T \)

For \( \neg A \lor B \):
- When \( A \) is True (T), \( \neg A \) is False (F). Thus, \( \neg A \lor B \) is equivalent to \( B \).
  - If \( B \) is True (T): \( F \lor T = T \)
  - If \( B \) is False (F): \( F \lor F = F \)
- When \( A \) is False (F), \( \neg A \) is True (T). Thus, \( \neg A \lor B \) is always True (T).

Comparing the truth values of both expressions:
- When \( A \) is True and \( B \) is True: Both are True.
- When \( A \) is True and \( B \) is False: Both are False.
- When \( A \) is False, regardless of \( B \): Both are True.

Since both expressions have the same truth values in all cases, they are logically equivalent. Additionally, this equivalence can be seen from the definition of material implication, where \( P \rightarrow Q \) is defined as \( \neg P \lor Q \).

Thus, we conclude that:

\[
A \rightarrow B \Leftrightarrow \neg A \lor B
\]

The final answer is \boxed{A \rightarrow B \Leftrightarrow \neg A \lor B}.

