llama Yes, I can help you with this proof.

In propositional logic, we can represent a conditional statement like "if A then B" using an implication operator (→) or an arrow. We also use the logical equivalence symbols = and ∨ (OR).

The statement to be proved is: A → B ≡ ~A ∨ B

To prove this, we need to demonstrate that both sides of the biconditional (≡) are logically equivalent.

**Step 1: Proving A → B ≢ ~A ∨ B**

To show this, we will use a proof by contradiction. We assume that the two statements are not logically equivalent:

∼(A → B) ∧ ∼(~A ∨ B)

Now, we can break down the double negation using De Morgan's laws and other logical equivalences.

**Step 2: Breaking down ~(~A ∨ B)**

Using De Morgan's law for double negation, we get:
~(~A ∨ B) = A ∧ ¬B
And applying the dual of the De Morgan's Law to (~A ∨ B):

~(A → B) ∧ (~A ∨ B)
= (∼A ∧ ~B) ∧ (~A ∨ B)

**Step 3: Using Distributive Property**

Now, we can distribute ~A over ~A ∨ B using the distributive property:

∼A ≡ ∼A ∧ true
∼(A → B) ≡ (∼A ∧ ~B) ∧ (∼A ∨ B)
= (∼A ∧ (~B ∧ ∼(A ∨ B)))
So, our first assumption (∼(A → B)) has become more complicated.

**Step 4: Breaking down ~(A ∨ B)**

Let's break this down using a truth table:

| A | B | A ∨ B |
| --- | --- | --- |
| T   | T   | T     |
| T   | F   | T     |
| F   | T   | T     |
| F   | F   | F     |

As we can see, A ∨ B is only false when both A and B are false. So:

~(A ∨ B) ≡ (A ∧ ¬B)

So the statement ~(A ∨ B) is true in all cases except when both A and B are false.

**Step 5: Using Distributive Property Again**

Using distributive property again we get:
= (∼A ∧ (~B ∧ ∼(A ∨ B)))
= (∼A ∧ (∼B ∧ (A ∧ ¬B)))
= (∼A ∧ ∼B ∧ A ∧ ¬B)

Now, this formula is true only when all the individual propositions are false. Since 'A' and 'B' appear twice in a different order, then this expression can be simplified to:

(A → B) ≡ ~(~A ∨ B)

So we have shown that ~(~A ∨ B) = A → B.

However there is still another way to prove the equality of these two statements. 

We also know (from other sources):

A → B ≡ ¬A ∨ B
Using our knowledge of material implication and biconditional we can say:

A → B ≡ ¬A ∨ B 
∴ (~A ∨ B) ≡ A → B
